test/Tests.lean
@@ -2,6 +2,7 @@
 Copyright (c) 2026 Paul Butcher. All rights reserved.
 Released under Apache 2.0 license as described in the file LICENSE.
 -/
+import Tests.Apple
 import Tests.Attempt
 import Tests.Consent
 import Tests.EndToEnd
